OneRuleAtATime.v
@@ -21,520 +21,522 @@ Section EnvUpdates.
   Proof.
     unfold commit_update; intros; rewrite fold_right_app; reflexivity.
   Qed.
+End EnvUpdates.
 
-  Section Semantics'.
-    Context {TVar: Type}.
-    Context {TFn: Type}.
+Section OneRuleAtATime.
+  Context {TVar: Type}.
+  Context {TFn: Type}.
 
-    Context {SigmaEnv: Env TFn ExternalFunction}.
-    Context {GammaEnv: Env TVar value}.
+  Context {RegEnv: Env nat bits}.
+  Context {SigmaEnv: Env TFn ExternalFunction}.
+  Context {GammaEnv: Env TVar value}.
 
-    Fixpoint interp_scheduler
-          (V: RegEnv.(env_t))
-          (Sigma: SigmaEnv.(env_t))
-          (sched_log: Log)
-          (s: scheduler TVar TFn)
-          {struct s} :=
-    match s with
-    | Done => Some ([], sched_log)
-    | Try r s1 s2 =>
-      match interp_rule V Sigma env_nil sched_log [] r with
-      | Success (l, _) => match interp_scheduler V Sigma (l ++ sched_log) s1 with
-                         | Some (rs, log) => Some (r :: rs, log)
-                         | None => None
-                         end
-      | CannotRun => interp_scheduler V Sigma sched_log s2
-      | Stuck => None
-      end
+  Fixpoint interp_scheduler_trace
+        (V: RegEnv.(env_t))
+        (Sigma: SigmaEnv.(env_t))
+        (sched_log: Log)
+        (s: scheduler TVar TFn)
+        {struct s} :=
+  match s with
+  | Done => Some ([], sched_log)
+  | Try r s1 s2 =>
+    match interp_rule V Sigma env_nil sched_log [] r with
+    | Success (l, _) => match interp_scheduler_trace V Sigma (l ++ sched_log) s1 with
+                       | Some (rs, log) => Some (r :: rs, log)
+                       | None => None
+                       end
+    | CannotRun => interp_scheduler_trace V Sigma sched_log s2
+    | Stuck => None
+    end
+  end.
+
+  Definition interp_scheduler_trace_and_update
+        (V: RegEnv.(env_t))
+        (Sigma: SigmaEnv.(env_t))
+        l
+        (s: scheduler TVar TFn) :=
+    match interp_scheduler_trace V Sigma l s with
+    | Some (rs, log) => Some (rs, commit_update V log)
+    | None => None
     end.
 
-    Definition interp_scheduler_and_update
-          (V: RegEnv.(env_t))
-          (Sigma: SigmaEnv.(env_t))
-          (s: scheduler TVar TFn)
-          l :=
-      match interp_scheduler V Sigma l s with
-      | Some (rs, log) => Some (rs, commit_update V log)
-      | None => None
-      end.
-
-    Definition update_one Sigma V r :=
-      match V with
-      | None => None
-      | Some V => match interp_scheduler_and_update V Sigma (Try r Done Done) [] with
-                 | Some (_, V') => Some V'
-                 | None => None
-                 end
-      end.
-
-    Definition latest_write l idx :=
-      log_find l idx (fun kind _ _ => match kind with
-                                   | LogWrite => true
-                                   | _ => false
-                                   end).
-
-    Lemma getenv_commit_update :
-      forall sl V idx val,
-        getenv V idx = Some val ->
-        getenv (commit_update V sl) idx =
-        match latest_write sl idx with
-        | Some {| val := val' |} => Some val'
-        | None => Some val
-        end.
-    Proof.
-      induction sl; cbn; intros.
-      - assumption.
-      - destruct a, kind, PeanoNat.Nat.eq_dec; subst;
-          try (erewrite IHsl by eassumption;
-               reflexivity).
-        + rewrite get_put_eq; reflexivity.
-        + rewrite get_put_neq by eauto.
-          erewrite IHsl by eassumption.
-          reflexivity.
-    Qed.
-
-    Lemma bool_result_Success :
-      forall b u,
-        bool_result b = Success u ->
-        b = true.
-    Proof.
-      destruct b; cbn; congruence.
-    Qed.
-
-    Require Import Ring_theory Ring Coq.setoid_ring.Ring.
-
-    Lemma log_forallb_app:
-      forall l l' reg (f: LogEntryKind -> Level -> bits -> bool),
-        log_forallb (l ++ l') reg f =
-        log_forallb l reg f && log_forallb l' reg f.
-    Proof.
-      unfold log_forallb.
-      intros; rewrite !forallb_app; reflexivity.
-    Qed.
-
-    Ltac set_forallb_fns :=
-      repeat match goal with
-             | [  |- context[log_forallb _ _ ?fn] ] =>
-               match fn with
-               | (fun _ => _) => set fn
+  Definition update_one Sigma V r :=
+    match V with
+    | None => None
+    | Some V => match interp_scheduler V Sigma [] (Try r Done Done) with
+               | Some log => Some (commit_update V log)
+               | None => None
                end
-             end.
+    end.
 
-    Lemma may_read0_app_sl :
-      forall sl sl' l idx,
-        may_read0 (sl ++ sl') l idx =
-        may_read0 sl l idx && may_read0 sl' l idx.
-    Proof.
-      unfold may_read0; intros.
-      rewrite !log_forallb_app.
-      ring_simplify.
-      f_equal.
-      f_equal.
-      rewrite <- !Bool.andb_assoc.
-      rewrite Bool.andb_diag; reflexivity.
-    Qed.
+  Definition latest_write l idx :=
+    log_find l idx (fun kind _ _ => match kind with
+                                 | LogWrite => true
+                                 | _ => false
+                                 end).
 
-    Lemma may_read1_app :
-      forall sl sl' idx,
-        may_read1 (sl ++ sl') idx =
-        may_read1 sl idx && may_read1 sl' idx.
-    Proof.
-      unfold may_read1; intros.
-      rewrite !log_forallb_app.
-      reflexivity.
-    Qed.
-
-    Lemma may_write_app_sl :
-      forall sl sl' l lvl idx,
-        may_write (sl ++ sl') l lvl idx =
-        may_write sl l lvl idx && may_write sl' l lvl idx.
-    Proof.
-      unfold may_write; intros.
-      destruct lvl; rewrite !log_forallb_app;
-        ring_simplify;
-        rewrite Bool.andb_diag;
+  Lemma getenv_commit_update :
+    forall sl V idx val,
+      getenv V idx = Some val ->
+      getenv (commit_update V sl) idx =
+      match latest_write sl idx with
+      | Some {| val := val' |} => Some val'
+      | None => Some val
+      end.
+  Proof.
+    unfold commit_update; induction sl; cbn; intros.
+    - assumption.
+    - destruct a, kind, PeanoNat.Nat.eq_dec; subst;
+        try (erewrite IHsl by eassumption;
+             reflexivity).
+      + rewrite get_put_eq; reflexivity.
+      + rewrite get_put_neq by eauto.
+        erewrite IHsl by eassumption.
         reflexivity.
-    Qed.
+  Qed.
 
-    Lemma log_find_in:
-      forall l idx P e,
-        log_find l idx P = Some e ->
-        List.In e l /\ e.(reg) = idx /\ P e.(kind) e.(level) e.(val) = true.
-    Proof.
-      unfold log_find; intros * H; destruct e; apply find_some in H.
-      destruct (PeanoNat.Nat.eq_dec idx reg); subst; cbn in *.
-      - intuition eauto.
-      - intuition discriminate.
-    Qed.
+  Lemma bool_result_Success :
+    forall b u,
+      bool_result b = Success u ->
+      b = true.
+  Proof.
+    destruct b; cbn; congruence.
+  Qed.
 
-    Lemma find_none_notb {A}:
-      forall (P: A -> bool) l,
-        (forall a, List.In a l -> P a = false) ->
-        find P l = None.
-    Proof.
-      induction l; cbn; intros * Hnot.
-      - reflexivity.
-      - pose proof (Hnot a).
-        destruct (P a); firstorder discriminate.
-    Qed.
+  Require Import Ring_theory Ring Coq.setoid_ring.Ring.
 
-    Ltac bool_step :=
-      match goal with
-      | _ => progress Common.bool_step
-      | [ H: log_forallb (_ ++ _) _ _ = _ |- _ ] =>
-        rewrite log_forallb_app in H
+  Lemma log_forallb_app:
+    forall l l' reg (f: LogEntryKind -> Level -> bits -> bool),
+      log_forallb (l ++ l') reg f =
+      log_forallb l reg f && log_forallb l' reg f.
+  Proof.
+    unfold log_forallb.
+    intros; rewrite !forallb_app; reflexivity.
+  Qed.
+
+  Ltac set_forallb_fns :=
+    repeat match goal with
+           | [  |- context[log_forallb _ _ ?fn] ] =>
+             match fn with
+             | (fun _ => _) => set fn
+             end
+           end.
+
+  Lemma may_read0_app_sl :
+    forall sl sl' l idx,
+      may_read0 (sl ++ sl') l idx =
+      may_read0 sl l idx && may_read0 sl' l idx.
+  Proof.
+    unfold may_read0; intros.
+    rewrite !log_forallb_app.
+    ring_simplify.
+    f_equal.
+    f_equal.
+    rewrite <- !Bool.andb_assoc.
+    rewrite Bool.andb_diag; reflexivity.
+  Qed.
+
+  Lemma may_read1_app :
+    forall sl sl' idx,
+      may_read1 (sl ++ sl') idx =
+      may_read1 sl idx && may_read1 sl' idx.
+  Proof.
+    unfold may_read1; intros.
+    rewrite !log_forallb_app.
+    reflexivity.
+  Qed.
+
+  Lemma may_write_app_sl :
+    forall sl sl' l lvl idx,
+      may_write (sl ++ sl') l lvl idx =
+      may_write sl l lvl idx && may_write sl' l lvl idx.
+  Proof.
+    unfold may_write; intros.
+    destruct lvl; rewrite !log_forallb_app;
+      ring_simplify;
+      rewrite Bool.andb_diag;
+      reflexivity.
+  Qed.
+
+  Lemma log_find_in:
+    forall l idx P e,
+      log_find l idx P = Some e ->
+      List.In e l /\ e.(reg) = idx /\ P e.(kind) e.(level) e.(val) = true.
+  Proof.
+    unfold log_find; intros * H; destruct e; apply find_some in H.
+    destruct (PeanoNat.Nat.eq_dec idx reg); subst; cbn in *.
+    - intuition eauto.
+    - intuition discriminate.
+  Qed.
+
+  Lemma find_none_notb {A}:
+    forall (P: A -> bool) l,
+      (forall a, List.In a l -> P a = false) ->
+      find P l = None.
+  Proof.
+    induction l; cbn; intros * Hnot.
+    - reflexivity.
+    - pose proof (Hnot a).
+      destruct (P a); firstorder discriminate.
+  Qed.
+
+  Ltac bool_step :=
+    match goal with
+    | _ => progress Common.bool_step
+    | [ H: log_forallb (_ ++ _) _ _ = _ |- _ ] =>
+      rewrite log_forallb_app in H
+    end.
+
+  Lemma may_read0_no_writes :
+    forall sl l idx,
+      may_read0 sl l idx = true ->
+      latest_write sl idx = None.
+  Proof.
+    unfold may_read0; intros.
+    repeat (cleanup_step || bool_step).
+    unfold log_forallb in *.
+    rewrite forallb_forall in *.
+    unfold latest_write, log_find.
+    apply find_none_notb.
+    intros a HIn.
+    repeat match goal with
+           | [ H: forall (_: LogEntry), _ |- _ ] => specialize (H a HIn)
+           end.
+    destruct a; cbn in *; destruct PeanoNat.Nat.eq_dec, kind; subst; try reflexivity.
+    destruct level; discriminate.
+  Qed.
+
+  Lemma find_app {A} :
+    forall sl sl' (P: A -> bool),
+      find P (sl ++ sl') =
+      match find P sl with
+      | Some e => Some e
+      | None => find P sl'
       end.
+  Proof.
+    induction sl; cbn; intros.
+    - reflexivity.
+    - destruct (P a); try rewrite IHsl; reflexivity.
+  Qed.
 
-    Lemma may_read0_no_writes :
-      forall sl l idx,
-        may_read0 sl l idx = true ->
-        latest_write sl idx = None.
-    Proof.
-      unfold may_read0; intros.
-      repeat (cleanup_step || bool_step).
-      unfold log_forallb in *.
-      rewrite forallb_forall in *.
-      unfold latest_write, log_find.
-      apply find_none_notb.
-      intros a HIn.
-      repeat match goal with
-             | [ H: forall (_: LogEntry), _ |- _ ] => specialize (H a HIn)
-             end.
-      destruct a; cbn in *; destruct PeanoNat.Nat.eq_dec, kind; subst; try reflexivity.
-      destruct level; discriminate.
-    Qed.
-
-    Lemma find_app {A} :
-      forall sl sl' (P: A -> bool),
-        find P (sl ++ sl') =
-        match find P sl with
-        | Some e => Some e
-        | None => find P sl'
-        end.
-    Proof.
-      induction sl; cbn; intros.
-      - reflexivity.
-      - destruct (P a); try rewrite IHsl; reflexivity.
-    Qed.
-
-    Lemma log_find_app :
-      forall sl sl' idx P,
-        log_find (sl ++ sl') idx P =
-        match log_find sl idx P with
-        | Some e => Some e
-        | None => log_find sl' idx P
-        end.
-    Proof.
-      unfold log_find; eauto using find_app.
-    Qed.
-
-    Lemma latest_write0_app :
-      forall sl sl' idx,
-        latest_write0 (sl ++ sl') idx =
-        match latest_write0 sl idx with
-        | Some e => Some e
-        | None => latest_write0 sl' idx
-        end.
-    Proof.
-      unfold latest_write0; eauto using log_find_app.
-    Qed.
-
-    Lemma assert_size_success :
-      forall v n v',
-        assert_size v n = Success v' ->
-        v = v' /\ length v' = n.
-    Proof.
-      unfold assert_size; intros; destruct PeanoNat.Nat.eq_dec;
-        firstorder (congruence || discriminate).
-    Qed.
-
-    Lemma assert_size_eq :
-      forall a n,
-        length a = n ->
-        assert_size a n = Success a.
-    Proof.
-      unfold assert_size; intros; destruct PeanoNat.Nat.eq_dec; firstorder.
-    Qed.
-
-    Lemma may_read1_latest_write_is_0 :
-      forall l idx,
-        may_read1 l idx = true ->
-        latest_write l idx = latest_write0 l idx.
-    Proof.
-      induction l.
-      - reflexivity.
-      - intros * H.
-        simpl in H.
-        repeat (bool_step || cleanup_step).
-        destruct a; cbn; destruct PeanoNat.Nat.eq_dec, kind; cbn;
-          try apply (IHl _ ltac:(eassumption)).
-        destruct level; cbn in *; try discriminate; reflexivity.
-    Qed.
-
-    Lemma fold_left2_result_failure {A B B': Type} (f: A -> B -> B' -> result A) :
-      forall (l: list B) (l': list B') (a0: result A),
-        a0 = CannotRun \/ a0 = Stuck ->
-        fold_left2 (fun acc b b' =>
-                      result_bind acc (fun acc =>
-                      f acc b b')) l l' a0 = a0.
-    Proof.
-      induction l; destruct 1; destruct l'; subst; cbn in *; eauto.
-    Qed.
-
-    Require Import TypeSafety.
-
-    Lemma log_write_consistent_latest_write :
-      forall l (v: fenv nat nat) idx e n,
-        log_write_consistent l v ->
-        fn v idx n ->
-        latest_write l idx = Some e ->
-        length (e.(val)) = n.
-    Proof.
-      intros * Hcst Hin Hwrt.
-      pose proof (log_find_in _ _ _ _ Hwrt); cbn in *.
-      repeat cleanup_step; destruct e, kind; cbn in *; try discriminate.
-      eauto using eq_sym.
-    Qed.
-
-    Ltac t_step :=
-      match goal with
-      | _ => cleanup_step
-      | [ H: context[may_read0 (_ ++ _) _ _] |- _ ] =>
-        rewrite may_read0_app_sl in H
-      | [ H: context[may_read1 (_ ++ _) _] |- _ ] =>
-        rewrite may_read1_app in H
-      | [ H: context[may_write (_ ++ _) _ _ _] |- _ ] =>
-        rewrite may_write_app_sl in H
-      | [ H: Success _ = Success _ |- _ ] =>
-        inversion H; subst; clear H
-      | [ H: bool_result _ = Success _ |- _ ] =>
-        apply bool_result_Success in H
-      | [ H: opt_result Stuck ?x = Success _ |- _ ] =>
-        destruct x eqn:?; subst; cbn in H; try discriminate
-      | [ H: result_bind ?x _ = Success _ |- _ ] =>
-        destruct x eqn:?; cbn in H; try discriminate
-      | [ H: result_map ?x _ = Success _ |- _ ] =>
-        destruct x eqn:?; cbn in H; try discriminate
-      | [ H: match ?x with _ => _ end = Success _ |- _ ] =>
-        destruct x eqn:?; subst; cbn in H; try discriminate
-      | [ H: assert_size _ _ = Success _ |- _ ] =>
-        apply assert_size_Success in H
-      | [ H: env_equiv (Env := ?Env) ?f ?tenv ?env,
-             H': getenv ?env ?k = Some ?v |- _ ] =>
-        pose_once (and_fst H k v) H'
-      | [ H: env_equiv ?f ?tenv ?env,
-             H': getenv ?env ?k = None |- _ ] =>
-        pose_once (and_snd H k) H'
-      | _ =>
-        bool_step
-      | [ H: match ?x with _ => _ end = ?c |- _ ] =>
-        let c_hd := constr_hd c in
-        is_constructor c_hd; destruct x eqn:?
-      | _ => progress (unfold assert_bits in *)
+  Lemma log_find_app :
+    forall sl sl' idx P,
+      log_find (sl ++ sl') idx P =
+      match log_find sl idx P with
+      | Some e => Some e
+      | None => log_find sl' idx P
       end.
+  Proof.
+    unfold log_find; eauto using find_app.
+  Qed.
 
-    Ltac t :=
-      repeat t_step.
+  Lemma latest_write0_app :
+    forall sl sl' idx,
+      latest_write0 (sl ++ sl') idx =
+      match latest_write0 sl idx with
+      | Some e => Some e
+      | None => latest_write0 sl' idx
+      end.
+  Proof.
+    unfold latest_write0; eauto using log_find_app.
+  Qed.
 
-    Lemma interp_rule_Success_call_consistent:
-      forall (args : list (rule TVar TFn)) (V : env_t RegEnv) (v : fenv nat nat)
-        (Sigma : env_t SigmaEnv) (Gamma : env_t GammaEnv) (sched_log rule_log l : Log) argvs,
-        env_equiv (length (A:=bool)) v V ->
-        log_write_consistent rule_log v ->
-        Forall
-          (fun r : rule TVar TFn =>
-             forall (V : env_t RegEnv) (v : fenv nat nat) (Sigma : env_t SigmaEnv)
-               (Gamma : env_t GammaEnv) (sl rule_log l : Log) (val : value),
-               env_equiv (length (A:=bool)) v V ->
-               log_write_consistent rule_log v ->
-               interp_rule V Sigma Gamma sl rule_log r = Success (l, val) -> log_write_consistent l v) args ->
-        forall (l1 : list bits) (argSizes : list nat),
-          length args = length argSizes ->
-          fold_left2_result
-            (fun '(rule_log, argvs) arg size =>
-            result_bind (interp_rule V Sigma Gamma sched_log rule_log arg) (fun '(rule_log, argv) =>
-            result_map (assert_bits argv size) (fun bs =>
-            (rule_log, bs :: argvs)))) args argSizes (rule_log, argvs) =
-          Success (l, l1) -> log_write_consistent l v.
-    Proof.
-      induction args; destruct argSizes; cbn in *; inversion 1; intros.
-      - t; eassumption.
-      - destruct interp_rule as [(?&[ | ?]) | | ] eqn:?; cbn in *.
-        + rewrite fold_left2_result_failure in H3; eauto || discriminate.
-        + unfold assert_size in *.
-          destruct PeanoNat.Nat.eq_dec; cbn in *.
-          * inversion H1; subst.
-            eapply (IHargs V v Sigma Gamma sched_log l0); eauto.
-          * rewrite fold_left2_result_failure in H3; eauto || discriminate.
-        + rewrite fold_left2_result_failure in H3; eauto || discriminate.
-        + rewrite fold_left2_result_failure in H3; eauto || discriminate.
-    Qed.
+  Lemma assert_size_success :
+    forall v n v',
+      assert_size v n = Success v' ->
+      v = v' /\ length v' = n.
+  Proof.
+    unfold assert_size; intros; destruct PeanoNat.Nat.eq_dec;
+      firstorder (congruence || discriminate).
+  Qed.
 
-    Lemma interp_rule_Success_consistent:
-      forall r {V v Sigma Gamma} sl rule_log l val,
-        env_equiv (@length bool) v V ->
-        log_write_consistent rule_log v ->
-        interp_rule V Sigma Gamma sl rule_log r = Success (l, val) ->
-        log_write_consistent l v.
-      induction r using rule_ind'; cbn; intros; try solve [t; eauto with types].
-      - t.
-        destruct a, sig; cbn in *.
-        eapply interp_rule_Success_call_consistent; eauto.
-    Qed.
+  Lemma assert_size_eq :
+    forall a n,
+      length a = n ->
+      assert_size a n = Success a.
+  Proof.
+    unfold assert_size; intros; destruct PeanoNat.Nat.eq_dec; firstorder.
+  Qed.
 
-    Lemma interp_rule_commit_call:
-      forall args : list (rule TVar TFn),
-        Forall
-          (fun r : rule TVar TFn =>
-             forall (V : env_t RegEnv) (v : fenv nat nat) (Sigma : env_t SigmaEnv)
-               (Gamma : env_t GammaEnv) (sl sl' rule_log l : Log) (val : value),
-               env_equiv (length (A:=bool)) v V ->
-               log_write_consistent sl v ->
-               log_write_consistent sl' v ->
-               interp_rule V Sigma Gamma (sl ++ sl') rule_log r = Success (l, val) ->
-               interp_rule (commit_update V sl') Sigma Gamma sl rule_log r = Success (l, val)) args ->
-        forall (V : env_t RegEnv) (Sigma : env_t SigmaEnv) (Gamma : env_t GammaEnv) (sl sl' rule_log l : Log)
-               (argSizes : list nat) v argvs,
-          length args = length argSizes ->
-          env_equiv (length (A:=bool)) v V ->
-          log_write_consistent sl v ->
-          log_write_consistent sl' v ->
-          forall l1 : list bits,
-            fold_left2_result
-              (fun '(rule_log, argvs) arg size =>
-                  result_bind (interp_rule V Sigma Gamma (sl ++ sl') rule_log arg) (fun '(rule_log, argv) =>
-                  result_map (assert_bits argv size) (fun bs =>
-                  (rule_log, bs :: argvs)))) args argSizes (rule_log, argvs) =
-            Success (l, l1) ->
-            fold_left2_result
-              (fun '(rule_log, argvs) arg size =>
-                  result_bind (interp_rule (commit_update V sl') Sigma Gamma sl rule_log arg) (fun '(rule_log, argv) =>
-                  result_map (assert_bits argv size) (fun bs =>
-                  (rule_log, bs :: argvs)))) args argSizes (rule_log, argvs) =
-            Success (l, l1).
-    Proof.
-      induction args; destruct argSizes; cbn in *; inversion 1; intros.
-      - t. reflexivity.
-      - destruct (interp_rule V Sigma Gamma (sl ++ sl') rule_log a) as [(? & ?) | | ] eqn:?; cbn in *.
-        + inversion H; subst.
-          eapply H8 in Heqr; eauto using log_write_consistent_nil.
-          rewrite Heqr; cbn.
-          destruct assert_bits; cbn in *.
-          * move IHargs at bottom.
-            unfold fold_left2_result in *.
-            eapply IHargs; eauto.
-          * rewrite fold_left2_result_failure in H5; eauto || discriminate.
-          * rewrite fold_left2_result_failure in H5; eauto || discriminate.
-        + rewrite fold_left2_result_failure in H5; eauto || discriminate.
-        + rewrite fold_left2_result_failure in H5; eauto || discriminate.
-    Qed.
+  Lemma may_read1_latest_write_is_0 :
+    forall l idx,
+      may_read1 l idx = true ->
+      latest_write l idx = latest_write0 l idx.
+  Proof.
+    induction l.
+    - reflexivity.
+    - intros * H.
+      simpl in H.
+      repeat (bool_step || cleanup_step).
+      destruct a; cbn; destruct PeanoNat.Nat.eq_dec, kind; cbn;
+        try apply (IHl _ ltac:(eassumption)).
+      destruct level; cbn in *; try discriminate; reflexivity.
+  Qed.
 
-    Lemma interp_rule_commit:
-      forall r {V v Sigma Gamma} sl sl' rule_log l val,
-        env_equiv (@length bool) v V ->
+  Lemma fold_left2_result_failure {A B B': Type} (f: A -> B -> B' -> result A) :
+    forall (l: list B) (l': list B') (a0: result A),
+      a0 = CannotRun \/ a0 = Stuck ->
+      fold_left2 (fun acc b b' =>
+                    result_bind acc (fun acc =>
+                    f acc b b')) l l' a0 = a0.
+  Proof.
+    induction l; destruct 1; destruct l'; subst; cbn in *; eauto.
+  Qed.
+
+  Require Import TypeSafety.
+
+  Lemma log_write_consistent_latest_write :
+    forall l (v: fenv nat nat) idx e n,
+      log_write_consistent l v ->
+      fn v idx n ->
+      latest_write l idx = Some e ->
+      length (e.(val)) = n.
+  Proof.
+    intros * Hcst Hin Hwrt.
+    pose proof (log_find_in _ _ _ _ Hwrt); cbn in *.
+    repeat cleanup_step; destruct e, kind; cbn in *; try discriminate.
+    eauto using eq_sym.
+  Qed.
+
+  Ltac t_step :=
+    match goal with
+    | _ => cleanup_step
+    | [ H: context[may_read0 (_ ++ _) _ _] |- _ ] =>
+      rewrite may_read0_app_sl in H
+    | [ H: context[may_read1 (_ ++ _) _] |- _ ] =>
+      rewrite may_read1_app in H
+    | [ H: context[may_write (_ ++ _) _ _ _] |- _ ] =>
+      rewrite may_write_app_sl in H
+    | [ H: Success _ = Success _ |- _ ] =>
+      inversion H; subst; clear H
+    | [ H: bool_result _ = Success _ |- _ ] =>
+      apply bool_result_Success in H
+    | [ H: opt_result Stuck ?x = Success _ |- _ ] =>
+      destruct x eqn:?; subst; cbn in H; try discriminate
+    | [ H: result_bind ?x _ = Success _ |- _ ] =>
+      destruct x eqn:?; cbn in H; try discriminate
+    | [ H: result_map ?x _ = Success _ |- _ ] =>
+      destruct x eqn:?; cbn in H; try discriminate
+    | [ H: match ?x with _ => _ end = Success _ |- _ ] =>
+      destruct x eqn:?; subst; cbn in H; try discriminate
+    | [ H: assert_size _ _ = Success _ |- _ ] =>
+      apply assert_size_Success in H
+    | [ H: env_related (Env := ?Env) ?f ?tenv ?env,
+           H': getenv ?env ?k = Some ?v |- _ ] =>
+      pose_once (and_fst H k v) H'
+    | [ H: env_related ?f ?tenv ?env,
+           H': getenv ?env ?k = None |- _ ] =>
+      pose_once (and_snd H k) H'
+    | _ =>
+      bool_step
+    | [ H: match ?x with _ => _ end = ?c |- _ ] =>
+      let c_hd := constr_hd c in
+      is_constructor c_hd; destruct x eqn:?
+    | _ => progress (unfold assert_bits in *)
+    end.
+
+  Ltac t :=
+    repeat t_step.
+
+  Lemma interp_rule_Success_call_consistent:
+    forall (args : list (rule TVar TFn)) (V : env_t RegEnv) (v : fenv nat nat)
+      (Sigma : env_t SigmaEnv) (Gamma : env_t GammaEnv) (sched_log rule_log l : Log) argvs,
+      env_related (length (A:=bool)) v V ->
+      log_write_consistent rule_log v ->
+      Forall
+        (fun r : rule TVar TFn =>
+           forall (V : env_t RegEnv) (v : fenv nat nat) (Sigma : env_t SigmaEnv)
+             (Gamma : env_t GammaEnv) (sl rule_log l : Log) (val : value),
+             env_related (length (A:=bool)) v V ->
+             log_write_consistent rule_log v ->
+             interp_rule V Sigma Gamma sl rule_log r = Success (l, val) -> log_write_consistent l v) args ->
+      forall (l1 : list bits) (argSizes : list nat),
+        length args = length argSizes ->
+        fold_left2_result
+          (fun '(rule_log, argvs) arg size =>
+          result_bind (interp_rule V Sigma Gamma sched_log rule_log arg) (fun '(rule_log, argv) =>
+          result_map (assert_bits argv size) (fun bs =>
+          (rule_log, bs :: argvs)))) args argSizes (rule_log, argvs) =
+        Success (l, l1) -> log_write_consistent l v.
+  Proof.
+    induction args; destruct argSizes; cbn in *; inversion 1; intros.
+    - t; eassumption.
+    - destruct interp_rule as [(?&[ | ?]) | | ] eqn:?; cbn in *.
+      + rewrite fold_left2_result_failure in H3; eauto || discriminate.
+      + unfold assert_size in *.
+        destruct PeanoNat.Nat.eq_dec; cbn in *.
+        * inversion H1; subst.
+          eapply (IHargs V v Sigma Gamma sched_log l0); eauto.
+        * rewrite fold_left2_result_failure in H3; eauto || discriminate.
+      + rewrite fold_left2_result_failure in H3; eauto || discriminate.
+      + rewrite fold_left2_result_failure in H3; eauto || discriminate.
+  Qed.
+
+  Lemma interp_rule_Success_consistent:
+    forall r {V v Sigma Gamma} sl rule_log l val,
+      env_related (@length bool) v V ->
+      log_write_consistent rule_log v ->
+      interp_rule V Sigma Gamma sl rule_log r = Success (l, val) ->
+      log_write_consistent l v.
+    induction r using rule_ind'; cbn; intros; try solve [t; eauto with types].
+    - t.
+      destruct a, sig; cbn in *.
+      eapply interp_rule_Success_call_consistent; eauto.
+  Qed.
+
+  Lemma interp_rule_commit_call:
+    forall args : list (rule TVar TFn),
+      Forall
+        (fun r : rule TVar TFn =>
+           forall (V : env_t RegEnv) (v : fenv nat nat) (Sigma : env_t SigmaEnv)
+             (Gamma : env_t GammaEnv) (sl sl' rule_log l : Log) (val : value),
+             env_related (length (A:=bool)) v V ->
+             log_write_consistent sl v ->
+             log_write_consistent sl' v ->
+             interp_rule V Sigma Gamma (sl ++ sl') rule_log r = Success (l, val) ->
+             interp_rule (commit_update V sl') Sigma Gamma sl rule_log r = Success (l, val)) args ->
+      forall (V : env_t RegEnv) (Sigma : env_t SigmaEnv) (Gamma : env_t GammaEnv) (sl sl' rule_log l : Log)
+             (argSizes : list nat) v argvs,
+        length args = length argSizes ->
+        env_related (length (A:=bool)) v V ->
         log_write_consistent sl v ->
         log_write_consistent sl' v ->
-        interp_rule V Sigma Gamma (sl ++ sl') rule_log r = Success (l, val) ->
-        interp_rule (commit_update V sl') Sigma Gamma sl rule_log r = Success (l, val).
-    Proof.
-      induction r using rule_ind'; cbn; intros V v Sigma Gamma * Heqiv Hcst Hcst'; intros; try congruence.
-      - (* Bind *)
-        t. erewrite IHr1; cbn; eauto.
-      - (* If *)
-        t;
-          erewrite IHr1; cbn; eauto;
-            [ erewrite IHr2; cbn; eauto |
-              erewrite IHr3; cbn; eauto ].
-      - destruct level.
-        + (* Read0 *)
-          t.
+        forall l1 : list bits,
+          fold_left2_result
+            (fun '(rule_log, argvs) arg size =>
+                result_bind (interp_rule V Sigma Gamma (sl ++ sl') rule_log arg) (fun '(rule_log, argv) =>
+                result_map (assert_bits argv size) (fun bs =>
+                (rule_log, bs :: argvs)))) args argSizes (rule_log, argvs) =
+          Success (l, l1) ->
+          fold_left2_result
+            (fun '(rule_log, argvs) arg size =>
+                result_bind (interp_rule (commit_update V sl') Sigma Gamma sl rule_log arg) (fun '(rule_log, argv) =>
+                result_map (assert_bits argv size) (fun bs =>
+                (rule_log, bs :: argvs)))) args argSizes (rule_log, argvs) =
+          Success (l, l1).
+  Proof.
+    induction args; destruct argSizes; cbn in *; inversion 1; intros.
+    - t. reflexivity.
+    - destruct (interp_rule V Sigma Gamma (sl ++ sl') rule_log a) as [(? & ?) | | ] eqn:?; cbn in *.
+      + inversion H; subst.
+        eapply H8 in Heqr; eauto using log_write_consistent_nil.
+        rewrite Heqr; cbn.
+        destruct assert_bits; cbn in *.
+        * move IHargs at bottom.
+          unfold fold_left2_result in *.
+          eapply IHargs; eauto.
+        * rewrite fold_left2_result_failure in H5; eauto || discriminate.
+        * rewrite fold_left2_result_failure in H5; eauto || discriminate.
+      + rewrite fold_left2_result_failure in H5; eauto || discriminate.
+      + rewrite fold_left2_result_failure in H5; eauto || discriminate.
+  Qed.
 
-          erewrite getenv_commit_update by eassumption.
-          destruct latest_write eqn:?; cbn.
-          * destruct l; cbn.
-            rewrite H1; cbn.
-            erewrite may_read0_no_writes in Heqo0; eauto.
-            discriminate.
+  Lemma interp_rule_commit:
+    forall r {V v Sigma Gamma} sl sl' rule_log l val,
+      env_related (@length bool) v V ->
+      log_write_consistent sl v ->
+      log_write_consistent sl' v ->
+      interp_rule V Sigma Gamma (sl ++ sl') rule_log r = Success (l, val) ->
+      interp_rule (commit_update V sl') Sigma Gamma sl rule_log r = Success (l, val).
+  Proof.
+    induction r using rule_ind'; cbn; intros V v Sigma Gamma * Heqiv Hcst Hcst'; intros; try congruence.
+    - (* Bind *)
+      t. erewrite IHr1; cbn; eauto.
+    - (* If *)
+      t;
+        erewrite IHr1; cbn; eauto;
+          [ erewrite IHr2; cbn; eauto |
+            erewrite IHr3; cbn; eauto ].
+    - destruct level.
+      + (* Read0 *)
+        t.
 
-          * rewrite H1; cbn.
-            reflexivity.
-
-        + (* Read1 *)
-          t;
-            rewrite app_assoc in Heqo0;
-            rewrite latest_write0_app in Heqo0;
-            t;
-            erewrite getenv_commit_update by eassumption.
-          destruct latest_write eqn:?; cbn.
-          * destruct l; cbn.
-            rewrite H2; cbn.
-
-            lazymatch goal with
-            | [ H: latest_write ?l ?idx = Some ?entry |- _ ] =>
-              let v0 := (eval cbn in entry.(Semantics.val)) in
-              change v0 with (entry.(Semantics.val));
-              erewrite log_write_consistent_latest_write
-            end; eauto.
-            rewrite assert_size_eq by auto; cbn.
-            reflexivity.
-          * rewrite H2; cbn.
-            rewrite assert_size_eq by auto; cbn.
-            reflexivity.
-          *
-
-            rewrite may_read1_latest_write_is_0 by eassumption.
-
-            rewrite Heqo0; cbn.
-            rewrite H2; cbn.
-            reflexivity.
-
-          * rewrite may_read1_latest_write_is_0 by eassumption.
-            rewrite Heqo0; cbn.
-            rewrite H1; cbn.
-            reflexivity.
-
-      - t.
         erewrite getenv_commit_update by eassumption.
         destruct latest_write eqn:?; cbn.
-        + destruct l; cbn.
-          erewrite IHr by eassumption; cbn.
+        * destruct l; cbn.
           rewrite H1; cbn.
+          erewrite may_read0_no_writes in Heqo0; eauto.
+          discriminate.
 
-            lazymatch goal with
-            | [ H: latest_write ?l ?idx = Some ?entry |- _ ] =>
-              let v0 := (eval cbn in entry.(Semantics.val)) in
-              change v0 with (entry.(Semantics.val));
-              erewrite log_write_consistent_latest_write
-            end; eauto.
-            rewrite assert_size_eq by auto; cbn.
-
+        * rewrite H1; cbn.
           reflexivity.
-        + erewrite IHr by eassumption; cbn.
-          rewrite H1; cbn.
+
+      + (* Read1 *)
+        t;
+          rewrite app_assoc in Heqo0;
+          rewrite latest_write0_app in Heqo0;
+          t;
+          erewrite getenv_commit_update by eassumption.
+        destruct latest_write eqn:?; cbn.
+        * destruct l; cbn.
+          rewrite H2; cbn.
+
+          lazymatch goal with
+          | [ H: latest_write ?l ?idx = Some ?entry |- _ ] =>
+            let v0 := (eval cbn in entry.(Semantics.val)) in
+            change v0 with (entry.(Semantics.val));
+            erewrite log_write_consistent_latest_write
+          end; eauto.
           rewrite assert_size_eq by auto; cbn.
           reflexivity.
+        * rewrite H2; cbn.
+          rewrite assert_size_eq by auto; cbn.
+          reflexivity.
+        *
 
-      - t.
-        destruct a, sig; cbn in *.
-        erewrite interp_rule_commit_call; cbn; eauto.
-    Qed.
+          rewrite may_read1_latest_write_is_0 by eassumption.
 
-  Lemma OneRuleAtATime:
-    forall Sigma s V v rs V' l0,
-      env_equiv (@length bool) v V ->
+          rewrite Heqo0; cbn.
+          rewrite H2; cbn.
+          reflexivity.
+
+        * rewrite may_read1_latest_write_is_0 by eassumption.
+          rewrite Heqo0; cbn.
+          rewrite H1; cbn.
+          reflexivity.
+
+    - t.
+      erewrite getenv_commit_update by eassumption.
+      destruct latest_write eqn:?; cbn.
+      + destruct l; cbn.
+        erewrite IHr by eassumption; cbn.
+        rewrite H1; cbn.
+
+          lazymatch goal with
+          | [ H: latest_write ?l ?idx = Some ?entry |- _ ] =>
+            let v0 := (eval cbn in entry.(Semantics.val)) in
+            change v0 with (entry.(Semantics.val));
+            erewrite log_write_consistent_latest_write
+          end; eauto.
+          rewrite assert_size_eq by auto; cbn.
+
+        reflexivity.
+      + erewrite IHr by eassumption; cbn.
+        rewrite H1; cbn.
+        rewrite assert_size_eq by auto; cbn.
+        reflexivity.
+
+    - t.
+      destruct a, sig; cbn in *.
+      erewrite interp_rule_commit_call; cbn; eauto.
+  Qed.
+
+  Lemma OneRuleAtATime':
+    forall V v Sigma s rs V' l0,
+      env_related (@length bool) v V ->
       log_write_consistent l0 v ->
-      interp_scheduler_and_update V Sigma s l0 = Some (rs, V') ->
+      interp_scheduler_trace_and_update V Sigma l0 s = Some (rs, V') ->
       List.fold_left (update_one Sigma) rs (Some (commit_update V l0)) = Some V'.
   Proof.
     induction s; cbn.
     - inversion 3; subst; cbn in *; eauto.
     - intros * Hequiv Hcst Heq.
-      unfold interp_scheduler_and_update in *; cbn in *.
+      unfold interp_scheduler_trace_and_update in *; cbn in *.
       destruct interp_rule as [(l & ?) | | ] eqn:?; try discriminate.
 
-      + destruct interp_scheduler as [(? & ?) | ] eqn:?; try discriminate;
+      + destruct interp_scheduler_trace as [(? & ?) | ] eqn:?; try discriminate;
           inversion Heq; subst; clear Heq; cbn.
-        unfold interp_scheduler_and_update; cbn.
+        unfold interp_scheduler_trace_and_update; cbn.
         enough (interp_rule (commit_update V l0) Sigma env_nil [] [] r = Success (l, v0)) as H.
         rewrite H.
         rewrite commit_update_assoc.
@@ -555,8 +557,38 @@ Section EnvUpdates.
       + eapply IHs2.
         eassumption.
         eassumption.
-        destruct interp_scheduler as [(? & ?) | ] eqn:?; try discriminate.
+        destruct interp_scheduler_trace as [(? & ?) | ] eqn:?; try discriminate.
         inversion Heq; subst.
         reflexivity.
   Qed.
-End Semantics'.
+
+  Lemma interp_scheduler_trace_correct :
+    forall V Sigma s l0 log,
+      interp_scheduler V Sigma l0 s = Some log ->
+      exists rs, interp_scheduler_trace V Sigma l0 s = Some (rs, log).
+  Proof.
+    induction s; cbn.
+    - inversion 1; subst; eauto.
+    - intros * Heq; destruct interp_rule as [(log' & ?) | | ] eqn:?.
+      + destruct (IHs1 _ _ Heq) as (rs & Heq').
+        rewrite Heq'; eauto.
+      + destruct (IHs2 _ _ Heq) as (rs & Heq').
+        rewrite Heq'; eauto.
+      + discriminate.
+  Qed.
+
+  Theorem OneRuleAtATime:
+    forall V Sigma s log,
+      interp_scheduler V Sigma [] s = Some log ->
+      exists rs, List.fold_left (update_one Sigma) rs (Some V) = Some (commit_update V log).
+  Proof.
+    intros * H.
+    apply interp_scheduler_trace_correct in H; destruct H as (rs & H).
+    exists rs.
+    (* change (Some V) with (Some (commit_update V [])). *)
+    eapply OneRuleAtATime' with (l0 := nil).
+    - eapply tenv_of_env_related.
+    - eapply log_write_consistent_nil.
+    - unfold interp_scheduler_trace_and_update; rewrite H; reflexivity.
+  Qed.
+End OneRuleAtATime.
